frodo/code/Hacl.Impl.Frodo.KEM.Encaps.fst
@@ -265,39 +265,6 @@ let crypto_kem_enc_ct_pack_c2 seed_e coins b sp_matrix c2 =
   clear_matrix v_matrix;
   pop_frame()
 
-#reset-options "--z3rlimit 50 --max_fuel 0 --max_ifuel 0"
-
-val lemma_update_ct:
-    c1:LSeq.lseq uint8 (v params_logq * v params_nbar * v params_n / 8)
-  -> c2:LSeq.lseq uint8 (v params_logq * v params_nbar * v params_nbar / 8)
-  -> d:LSeq.lseq uint8 (v crypto_bytes)
-  -> ct:LSeq.lseq uint8 (v crypto_ciphertextbytes)
-  -> Lemma
-    (requires (
-      let c1Len = v params_logq * v params_nbar * v params_n / 8 in
-      let c2Len = v params_logq * v params_nbar * v params_nbar / 8 in
-      Spec.Frodo.KEM.expand_crypto_ciphertextbytes ();
-      LSeq.sub ct 0 c1Len == c1 /\
-      LSeq.sub ct c1Len c2Len == c2 /\
-      LSeq.sub ct (c1Len + c2Len) (v crypto_bytes) == d))
-    (ensures ct == LSeq.concat (LSeq.concat c1 c2) d)
-let lemma_update_ct c1 c2 d ct =
-  let ct1 = LSeq.concat (LSeq.concat c1 c2) d in
-  let c1Len = v params_logq * v params_nbar * v params_n / 8 in
-  let c2Len = v params_logq * v params_nbar * v params_nbar / 8 in
-  Spec.Frodo.KEM.expand_crypto_ciphertextbytes ();
-
-  FStar.Seq.Base.lemma_eq_intro (LSeq.sub ct1 0 c1Len) c1;
-  FStar.Seq.Base.lemma_eq_intro (LSeq.sub ct1 c1Len c2Len) c2;
-  FStar.Seq.Base.lemma_eq_intro (LSeq.sub ct1 (c1Len + c2Len) (v crypto_bytes)) d;
-
-  FStar.Seq.Properties.lemma_split (LSeq.sub ct 0 (c1Len + c2Len)) c1Len;
-  FStar.Seq.Properties.lemma_split (LSeq.sub ct1 0 (c1Len + c2Len)) c1Len;
-  FStar.Seq.Properties.lemma_split ct (c1Len + c2Len);
-  FStar.Seq.Properties.lemma_split ct1 (c1Len + c2Len)
-
-#reset-options "--z3rlimit 50 --max_fuel 0 --max_ifuel 0 --using_facts_from '* -FStar.Seq'"
-
 inline_for_extraction noextract
 val crypto_kem_enc_ct_inner:
     seed_a:lbytes bytes_seed_a
@@ -341,7 +308,8 @@ let crypto_kem_enc_ct_inner seed_a seed_e b coins sp_matrix d ct =
   let h3 = ST.get () in
   LSeq.eq_intro (LSeq.sub #_ #(v crypto_ciphertextbytes) (as_seq h3 ct) (v c1Len) (v c2Len)) (as_seq h2 c2);
   LSeq.eq_intro (LSeq.sub #_ #(v crypto_ciphertextbytes) (as_seq h3 ct) 0 (v c1Len)) (as_seq h1 c1);
-  lemma_update_ct (as_seq h3 c1) (as_seq h3 c2) (as_seq h0 d) (as_seq h3 ct)
+
+  LSeq.lemma_concat3 (v c1Len) (as_seq h3 c1) (v c2Len) (as_seq h3 c2) (v crypto_bytes) (as_seq h0 d) (as_seq h3 ct)
 
 val crypto_kem_enc_ct:
     pk:lbytes crypto_publickeybytes
@@ -370,24 +338,6 @@ let crypto_kem_enc_ct pk g coins ct =
   clear_matrix sp_matrix;
   pop_frame()
 
-#reset-options "--z3rlimit 50 --max_fuel 0 --max_ifuel 0"
-
-val lemma_update_ss_init:
-    c12:LSeq.lseq uint8 (v crypto_ciphertextbytes - v crypto_bytes)
-  -> kd:LSeq.lseq uint8 (2 * v crypto_bytes)
-  -> ss_init:LSeq.lseq uint8 (v crypto_ciphertextbytes + v crypto_bytes)
-  -> Lemma
-    (requires
-      LSeq.sub ss_init 0 (v crypto_ciphertextbytes - v crypto_bytes) == c12 /\
-      LSeq.sub ss_init (v crypto_ciphertextbytes - v crypto_bytes) (2 * v crypto_bytes) == kd)
-    (ensures ss_init == LSeq.concat c12 kd)
-let lemma_update_ss_init c12 kd ss_init =
-  let ss_init1 = LSeq.concat c12 kd in
-  FStar.Seq.Properties.lemma_split ss_init (v crypto_ciphertextbytes - v crypto_bytes);
-  FStar.Seq.Properties.lemma_split ss_init1 (v crypto_ciphertextbytes - v crypto_bytes)
-
-#reset-options "--z3rlimit 50 --max_fuel 0 --max_ifuel 0 --using_facts_from '* -FStar.Seq'"
-
 val crypto_kem_enc_ss:
     g:lbytes (size 3 *! crypto_bytes)
   -> ct:lbytes crypto_ciphertextbytes
@@ -405,34 +355,9 @@ let crypto_kem_enc_ss g ct ss =
   let ss_init:lbytes ss_init_len = create ss_init_len (u8 0) in
   let c12 = sub ct (size 0) (crypto_ciphertextbytes -! crypto_bytes) in
   let kd = sub #uint8 #_ #(2 * v crypto_bytes) g crypto_bytes (size 2 *! crypto_bytes) in
-  let h0 = ST.get () in
-  update_sub ss_init (size 0) (crypto_ciphertextbytes -! crypto_bytes) c12;
-  update_sub ss_init (crypto_ciphertextbytes -! crypto_bytes) (size 2 *! crypto_bytes) kd;
-  let h2 = ST.get () in
-  LSeq.eq_intro (LSeq.sub #_ #(v ss_init_len) (as_seq h2 ss_init) 0 (v crypto_ciphertextbytes - v crypto_bytes)) (as_seq h0 c12);
-  lemma_update_ss_init (as_seq h0 c12) (as_seq h0 kd) (as_seq h2 ss_init);
-  //assert (as_seq h2 ss_init == S.update_ss_init (as_seq h0 c12) (as_seq h0 kd) (as_seq h0 ss_init));
+  concat2 (crypto_ciphertextbytes -! crypto_bytes) c12 (size 2 *! crypto_bytes) kd ss_init;
   cshake_frodo ss_init_len ss_init (u16 7) crypto_bytes ss;
   pop_frame()
-
-#reset-options "--z3rlimit 50 --max_fuel 0 --max_ifuel 0"
-
-val lemma_update_pk_coins:
-    pk:LSeq.lseq uint8 (v crypto_publickeybytes)
-  -> coins:LSeq.lseq uint8 (v params_nbar * v params_nbar * v params_extracted_bits / 8)
-  -> pk_coins:LSeq.lseq uint8 (v crypto_publickeybytes + v params_nbar * v params_nbar * v params_extracted_bits / 8)
-  -> Lemma
-    (requires
-      LSeq.sub pk_coins 0 (v crypto_publickeybytes) == pk /\
-      LSeq.sub pk_coins (v crypto_publickeybytes)
-	(v params_nbar * v params_nbar * v params_extracted_bits / 8) == coins)
-    (ensures pk_coins == LSeq.concat pk coins)
-let lemma_update_pk_coins pk coins pk_coins =
-  let pk_coins1 = LSeq.concat pk coins in
-  FStar.Seq.Properties.lemma_split pk_coins (v crypto_publickeybytes);
-  FStar.Seq.Properties.lemma_split pk_coins1 (v crypto_publickeybytes)
-
-#reset-options "--z3rlimit 50 --max_fuel 0 --max_ifuel 0 --using_facts_from '* -FStar.Seq'"
 
 inline_for_extraction noextract
 val crypto_kem_enc_0:
@@ -449,12 +374,7 @@ val crypto_kem_enc_0:
 let crypto_kem_enc_0 coins pk g =
   push_frame();
   let pk_coins:lbytes (crypto_publickeybytes +! bytes_mu) = create (crypto_publickeybytes +! bytes_mu) (u8 0) in
-  let h0 = ST.get () in
-  update_sub pk_coins (size 0) crypto_publickeybytes pk;
-  update_sub pk_coins crypto_publickeybytes bytes_mu coins;
-  let h2 = ST.get () in
-  LSeq.eq_intro (LSeq.sub #_ #(v crypto_publickeybytes + v bytes_mu) (as_seq h2 pk_coins) 0 (v crypto_publickeybytes)) (as_seq h0 pk);
-  lemma_update_pk_coins (as_seq h0 pk) (as_seq h0 coins) (as_seq h2 pk_coins);
+  concat2 crypto_publickeybytes pk bytes_mu coins pk_coins;
   cshake_frodo (crypto_publickeybytes +! bytes_mu) pk_coins (u16 3) (size 3 *! crypto_bytes) g;
   pop_frame()
 
@@ -498,7 +418,7 @@ val crypto_kem_enc_:
 let crypto_kem_enc_ coins ct ss pk =
   push_frame();
   let g:lbytes (size 3 *! crypto_bytes) = create (size 3 *! crypto_bytes) (u8 0) in
-  crypto_kem_enc_0 coins pk g;  
+  crypto_kem_enc_0 coins pk g;
   crypto_kem_enc_1 g coins ct ss pk;
   pop_frame()
 
