lib/fst/Lib.Buffer.fst
@@ -110,6 +110,26 @@ let update_sub_f #a #len h0 buf start n spec f =
   B.modifies_buffer_elim (sub #_ #len #(len - v start - v n) buf (start +! n) (size len -. start -. n)) (B.loc_buffer tmp) h0 h1;
   Sequence.lemma_update_sub #a #len (B.as_seq h0 buf) (v start) (v n) (spec h0) (B.as_seq h1 buf)
 
+let concat2 #a len0 s0 len1 s1 s =
+  let h0 = ST.get () in
+  update_sub s (size 0) len0 s0;
+  update_sub s len0 len1 s1;
+  let h1 = ST.get () in
+  Seq.eq_intro (Seq.sub (as_seq h1 s) 0 (v len0)) (as_seq h0 s0);
+  Seq.lemma_concat2 (v len0) (as_seq h0 s0) (v len1) (as_seq h0 s1) (as_seq h1 s)
+
+let concat3 #a len0 s0 len1 s1 len2 s2 s =
+  let h0 = ST.get () in
+  update_sub s (size 0) len0 s0;
+  update_sub s len0 len1 s1;
+  let h1 = ST.get () in
+  Seq.eq_intro (Seq.sub (as_seq h1 s) 0 (v len0)) (as_seq h0 s0);
+  update_sub s (len0 +! len1) len2 s2;
+  let h2 = ST.get () in
+  Seq.eq_intro (Seq.sub (as_seq h2 s) 0 (v len0)) (as_seq h0 s0);
+  Seq.eq_intro (Seq.sub (as_seq h2 s) (v len0) (v len1)) (as_seq h0 s1);
+  Seq.lemma_concat3 (v len0) (as_seq h0 s0) (v len1) (as_seq h0 s1) (v len2) (as_seq h0 s2) (as_seq h2 s)
+
 let loop_nospec #h0 #a #len n buf impl =
   let inv h1 j = B.modifies (B.loc_buffer buf) h0 h1 in
   Lib.Loops.for (size 0) n inv impl
@@ -243,13 +263,12 @@ let loop_blocks #a #b #blen bs inpLen inp spec_f spec_l f l w =
   l rem last w
 
 
-let mapT #a #b #len o clen f inp = 
+let mapT #a #b #len o clen f inp =
   let h0 = ST.get () in
   loop_nospec #h0 clen o (fun i -> o.(i) <- f inp.(i));
   admit()
 
-let imapT #a #b #len o clen f inp = 
+let imapT #a #b #len o clen f inp =
   let h0 = ST.get () in
   loop_nospec #h0 clen o (fun i -> o.(i) <- f (iindex inp i));
   admit()
-
